BlockCacheSystem/BetreeJournalSystem.i.dfy
@@ -1,0 +1,86 @@
+include "BetreeSystem.i.dfy"
+include "JournalSystem.i.dfy"
+include "BetreeSystem_Refines_StatesViewMap.i.dfy"
+include "JournalSystem_Refines_JournalView.i.dfy"
+
+module BetreeJournalSystem {
+  import BS = BetreeSystem
+  import JS = JournalSystem
+
+  //import BlockSystemRef = BlockSystem_Refines_StatesView
+  import BetreeSystemRef = BetreeSystem_Refines_StatesViewMap
+  import JournalSystemRef = JournalSystem_Refines_JournalView
+  import CompositeView
+
+  datatype Constants = Constants(bs: BS.Constants, js: JS.Constants)
+  datatype Variables = Variables(bs: BS.Variables, js: JS.Variables)
+
+  predicate Init(k: Constants, s: Variables)
+  {
+    exists loc ::
+      && BS.Init(k.bs, s.bs, loc)
+      && JS.Init(k.js, s.js, loc)
+  }
+
+  predicate Next(k: Constants, s: Variables, s': Variables)
+  {
+    exists vop ::
+      && BS.Next(k.bs, s.bs, s'.bs, vop)
+      && JS.Next(k.js, s.js, s'.js, vop)
+  }
+
+  function Ik(k: Constants) : CompositeView.Constants {
+    CompositeView.Constants(
+      BetreeSystemRef.Ik(k.bs),
+      JournalSystemRef.Ik(k.js)
+    )
+  }
+
+  function I(k: Constants, s: Variables) : CompositeView.Variables {
+    CompositeView.Variables(
+      BetreeSystemRef.I(k.bs, s.js),
+      JournalSystemRef.I(k.bs, s.js)
+    )
+  }
+
+  predicate Inv(k: Constants, s: Variables)
+  {
+    && BS.Inv(k.bs, s.bs)
+    && JS.Inv(k.js, s.js)
+    //&& JS.PersistentLoc(s.js) in BS.BetreeDisk(k.bs, s.bs)
+    && CompositeView.Inv(Ik(k), I(s))
+  }
+
+  lemma InitImpliesInv(k: Constants, s: Variables)
+  requires Init(k, s)
+  ensures Inv(k, s)
+  {
+    var loc :|
+      && BS.Init(k.bs, s.bs, loc)
+      && JS.Init(k.js, s.js, loc);
+    BS.InitImpliesInv(k.bs, s.bs, loc);
+    JS.InitImpliesInv(k.js, s.js, loc);
+  }
+
+  lemma NextImpliesInv(k: Constants, s: Variables, s': Variables)
+  requires Inv(k, s)
+  requires Next(k, s, s')
+  ensures Inv(k, s')
+  {
+    var vop :|
+      && BS.Next(k.bs, s.bs, s'.bs, vop)
+      && JS.Next(k.js, s.js, s'.js, vop);
+    BS.NextPreservesInv(k.bs, s.bs, s'.bs, vop);
+    JS.NextPreservesInv(k.js, s.js, s'.js, vop);
+
+    //var step :| BS.NextStep(k.bs, s.bs, s'.bs, vop);
+    //BlockSystemRef.StepGraphs(k.bs, s.bs, s'.bs, vop
+
+  }
+
+  lemma InvImpliesPersistentLocInGraph(k: Constants, s: Variables)
+  requires Inv(k, s)
+  ensures JS.PersistentLoc(s.js) in BS.BetreeDisk(k.bs, s.bs)
+  {
+  }
+}
